code/Yazi.LZ77.fst
@@ -1,0 +1,62 @@
+module Yazi.LZ77
+
+module B = LowStar.Buffer
+module Cast = FStar.Int.Cast
+module CB = LowStar.ConstBuffer
+module ST = FStar.HyperStack.ST
+module U16 = FStar.UInt16
+module U32 = FStar.UInt32
+module U8 = FStar.UInt8
+
+open LowStar.BufferOps
+open FStar.Mul
+open Spec.LZ77
+
+let context_valid (c: lz77_context) =
+  let open U16 in
+  is_window_bits (v c.w_bits) /\
+  is_window_mask (v c.w_bits) (v c.w_mask) /\
+  is_window_size (v c.w_bits) (U32.v c.w_size) /\
+  (U32.v c.window_size) == (U32.v c.w_size) * 2 /\
+  B.length c.window == U32.v c.window_size /\
+  B.length c.prev == U32.v c.w_size /\
+  is_hash_bits (v c.h_bits) /\
+  is_hash_size (v c.h_bits) (U32.v c.h_size) /\
+  is_hash_mask (v c.h_bits) (v c.h_mask) /\
+  is_hash_shift (v c.h_bits) (v c.shift) /\
+  B.length c.head == U32.v c.h_size
+
+#set-options "--fuel 0 --ifuel 0"
+inline_for_extraction
+let update_hash
+  (a b c: Ghost.erased U8.t)
+  (ctx: CB.const_buffer lz77_context)
+  (ins_h: B.pointer U16.t)
+  (d: U8.t):
+  ST.StackInline unit
+  (ensures fun h ->
+    let open U16 in
+    let ctx' = CB.as_mbuf ctx in
+    CB.length ctx == 1 /\
+    (let ctx'' = B.get h ctx' 0 in
+    CB.live h ctx /\ B.live h ins_h /\
+    B.disjoint ctx' ins_h /\
+    context_valid ctx'' /\
+    is_rolling_hash (v ctx''.h_bits) a b c (B.get h ins_h 0)))
+  (requires fun h0 _ h1 ->
+    let open U16 in
+    let ctx' = B.get h1 (CB.as_mbuf ctx) 0 in
+    let h = B.get h1 ins_h 0 in
+    B.modifies (B.loc_buffer ins_h) h0 h1 /\
+    is_rolling_hash (v ctx'.h_bits) b c d h) =
+  let open U16 in
+  let d' = Cast.uint8_to_uint16 d in
+  let bits = (CB.index ctx 0ul).h_bits in
+  let bits': Ghost.erased hash_bits = Ghost.hide (v bits) in
+  let s = (CB.index ctx 0ul).shift in
+  let m = (CB.index ctx 0ul).h_mask in
+  let s' = Cast.uint16_to_uint32 s in
+  let h = !*ins_h in
+  let h' = ((h <<^ s') ^^ d') &^ m in
+  roll_hash_eq bits' m s a b c d h;
+  ins_h *= h'
