specs/Spec.LZ77.fst
@@ -1,0 +1,78 @@
+module Spec.LZ77
+
+module Cast = FStar.Int.Cast
+module U16 = FStar.UInt16
+module U32 = FStar.UInt32
+module UInt = FStar.UInt
+
+open FStar.Mul
+open Lib.UInt
+
+unfold let (^) #n = UInt.logxor #n
+unfold let (&@) #n = UInt.logand #n
+unfold let (<<) #n = UInt.shift_left #n
+
+#set-options "--fuel 4 --ifuel 4"
+let triple_shift_zero
+  (#n: hash_bits)
+  (shift: hash_shift n)
+  (mask: hash_mask n)
+  (a: U8.t): Lemma
+  (ensures (((U16.v (Cast.uint8_to_uint16 a)) << (3 * shift)) &@ mask) == 0) =
+  assert(3 * shift >= n);
+  hash_mask_ones n;
+  let a' = (U16.v (Cast.uint8_to_uint16 a)) << (3 * shift) in
+  assert(Seq.equal (UInt.to_vec (a' &@ mask)) (UInt.to_vec (UInt.zero 16)))
+
+#set-options "--fuel 0 --ifuel 0"
+let roll_hash_eq bits m s a b c d h =
+  let open U16 in
+  let m' = v m in
+  let s' = v s in
+  let a' = Cast.uint8_to_uint16 a in
+  let b' = Cast.uint8_to_uint16 b in
+  let c' = Cast.uint8_to_uint16 c in
+  let d' = Cast.uint8_to_uint16 d in
+  let a'' = v a' in
+  let b'' = v b' in
+  let c'' = v c' in
+  let d'' = v d' in
+  let h' = ((h <<^ (Cast.uint16_to_uint32 s)) ^^ d') &^ m in
+  UInt.shift_left_logand_lemma (((a'' << (2 * s')) ^ (b'' << s')) ^ c'') m' s';
+  UInt.shift_left_logxor_lemma ((a'' << (2 * s')) ^ (b'' << s')) c'' s';
+  UInt.shift_left_logxor_lemma (a'' << (2 * s')) (b'' << s') s';
+  logxor_logand_distr
+    ((((a'' << (3 * s')) ^ (b'' << (2 * s'))) ^ (c'' << s')) &@ (m' << s'))
+    d''
+    m';
+  UInt.logand_associative
+    (((a'' << (3 * s')) ^ (b'' << (2 * s'))) ^ (c'' << s'))
+    (m' << s')
+    m';
+  UInt.logand_commutative (m' << s') m';
+  UInt.logand_associative
+    (((a'' << (3 * s')) ^ (b'' << (2 * s'))) ^ (c'' << s'))
+    m'
+    (m' << s');
+  logxor_logand_distr
+    ((a'' << (3 * s')) ^ (b'' << (2 * s')))
+    (c'' << s')
+    m';
+  logxor_logand_distr (a'' << (3 * s')) (b'' << (2 * s')) m';
+  triple_shift_zero #bits s' m' a;
+  UInt.logxor_commutative 0 ((b'' << (2 * s')) &@ m');
+  UInt.logxor_lemma_1 ((b'' << (2 * s')) &@ m');
+  logxor_logand_distr (b'' << (2 * s')) (c'' << s') m';
+  shift_left_append b'' s' s';
+  UInt.shift_left_logxor_lemma (b'' << s') c'' s';
+  UInt.logand_associative (((b'' << s') ^ c'') << s') m' (m' << s');
+  UInt.logand_associative (((b'' << s') ^ c'') << s') (m' << s') m';
+  UInt.shift_left_logand_lemma ((b'' << s') ^ c'') m' s';
+  logxor_logand_distr ((((b'' << s') ^ c'') &@ m') << s') d'' m';
+  assert(forall (i: nat{i < 16}).
+    UInt.nth (((((b'' << s') ^ c'') &@ m') << s') &@ m') i ==
+    UInt.nth ((((b'' << s') ^ c'') << s') &@ m') i);
+  UInt.to_vec_lemma_2
+    (((((b'' << s') ^ c'') &@ m') << s') &@ m')
+    ((((b'' << s') ^ c'') << s') &@ m');
+  logxor_logand_distr (((b'' << s') ^ c'') << s') d'' m'
